Cpc/Proofs/RuleSupport/DtConsEqSupport.lean
@@ -1663,7 +1663,7 @@ private theorem dtConsSpineRoot_apply_generic
           | root s d i =>
               rfl
           | app x''' hSp'' =>
-              rfl
+              cases hSp'' <;> rfl
 
 private inductive CtorSpineRoot : Term -> Term -> Prop where
   | tuple :
@@ -1712,7 +1712,9 @@ private theorem ctorSpineRoot_apply_generic_of_not_tuple_one_arg
       | dtCons s d i =>
           rfl
       | app y hPrev' =>
-          cases hPrev' <;> rfl
+          cases hPrev' <;> try rfl
+          case app z hPrev'' =>
+            cases hPrev'' <;> rfl
 
 private theorem ctorSpineRoot_to_smt_ne_dt_sel
     {f root : Term}
